src/Stream.v
@@ -91,10 +91,10 @@ Proof.
   now rewrite from_S.
 Qed.
 
-Notation "（ s , n ） ⊨ P" := (P (from n s)) (at level 85).
+Notation "[ s , n ]  ⊨ P" := (P (from n s)) (at level 85).
 
-Definition every (P : Stream -> Prop) (s : Stream) := forall i,（s, i）⊨ P.
-Definition any   (P : Stream -> Prop) (s : Stream) := exists i,（s, i）⊨ P.
+Definition every (P : Stream -> Prop) (s : Stream) := forall i, [s, i] ⊨ P.
+Definition any   (P : Stream -> Prop) (s : Stream) := exists i, [s, i] ⊨ P.
 
 Section stream_eq_coind.
   Variable R : Stream -> Stream -> Prop.
@@ -280,7 +280,7 @@ Arguments tail {a} s.
 Arguments every {a} P s.
 Arguments any {a} P s.
 
-Notation "（ s , n ） ⊨ P" := (P (from n s)) (at level 75).
+Notation "[ s , n ]  ⊨ P" := (P (from n s)) (at level 75).
 
 CoFixpoint constant {a : Type} (x : a) : Stream a := Cons x (constant x).
 
